feat(lts): WIP -- sim_traces proof

theories/common/utils.v
@@ -253,7 +253,7 @@ End OptionUtils.
 
 Section SeqUtils.
 Context {T : Type}.
-Implicit Types (s : seq T).
+Implicit Types (x : T) (s : seq T).
 
 (* copy-paste of Tauto.ocons *)
 Definition ocons o s := 
@@ -262,10 +262,29 @@ Definition ocons o s :=
   | None   => s
   end.
 
+Lemma rcons0 x : 
+  rcons [::] x = [:: x].
+Proof. done. Qed.
+
+Lemma behead_rcons x s :
+  behead (rcons s x) = if nilp s then [::] else rcons (behead s) x.
+Proof. case: s=> //=. Qed.
+
 End SeqUtils. 
 
 Section TupleUtils.
 Context {T : Type}.
+
+Definition tlast n (t : n.+1.-tuple T) : T := tnth t ord_max. 
+
+Lemma thead_head x n (t : n.+1.-tuple T) : thead t = head x t.
+Proof. by rewrite /thead (tnth_nth x). Qed.
+
+Lemma tlast_last x n (t : n.+1.-tuple T) : tlast t = last x t.
+Proof. by rewrite /tlast (tnth_nth x) -nth_last size_tuple /=. Qed.
+
+Lemma tlast_rcons n (t : n.-tuple T) x : tlast [tuple of rcons t x] = x.
+Proof. by rewrite (tlast_last x) last_rcons. Qed.
 
 (* TODO: duplicate of https://github.com/math-comp/math-comp/pull/777 *)
 Lemma val_tcast m n (eq_mn : m = n) (t : m.-tuple T) :
