theories/concur/lts.v
@@ -1,5 +1,6 @@
 From RelationAlgebra Require Import lattice monoid rel.
-From mathcomp Require Import ssreflect ssrfun ssrbool ssrnat eqtype seq path. 
+From mathcomp Require Import ssreflect ssrfun ssrbool ssrnat eqtype.
+From mathcomp Require Import seq tuple path.
 From eventstruct Require Import utils relalg.
 
 (******************************************************************************)
@@ -190,7 +191,7 @@ Structure trace : Type := Trace {
 
 Canonical trace_subType := Eval hnf in [subType for trace_val].
 
-Implicit Types (tr : trace).
+Implicit Types (ts : trace_seq S) (tr : trace).
 
 Lemma trace_steps tr : all is_step tr.
 Proof. by case: tr; rewrite /is_trace=> ? /= /andP[]. Qed.
@@ -198,29 +199,39 @@ Proof. by case: tr; rewrite /is_trace=> ? /= /andP[]. Qed.
 Lemma trace_lnk tr : sorted lnk tr.
 Proof. by case: tr; rewrite /is_trace=> ? /= /andP[]. Qed.
 
-(* TODO: better name? *)
-Definition joint : rel (trace_seq S) := 
-  fun s1 s2 => 
-    match s2 with 
-    | [::]     => true
-    | st :: s2 => lnk (last (rev_step st) s1) st
-    end.
-
 Definition labels : trace_seq S -> seq L := map lbl. 
 
-Definition states : trace_seq S -> seq S := 
-  fun s => 
-    match s with 
-    | [::]    => [::]
-    | st :: s => src st :: dst st :: map dst s
+Definition states : S -> trace_seq S -> seq S := 
+  fun s ts => 
+    match ts with 
+    | [::]    => [:: s]
+    | st :: _ => src st :: map dst ts
     end. 
 
+Lemma size_states s ts : size (states s ts) == (size ts).+1.
+Proof. by rewrite /states; case: ts=> [|??] //=; rewrite size_map. Qed.
+Canonical states_tuple s ts := Tuple (size_states s ts).
+
+Definition fst_state : S -> trace_seq S -> S := 
+  fun s ts => thead [tuple of states s ts].
+
+Definition lst_state : S -> trace_seq S -> S := 
+  fun s ts => tlast [tuple of states s ts].  
+
 Definition traces_at : S -> pred trace := 
-  fun s tr => s == head s (states tr).
+  fun s tr => s == fst_state s tr.
 
 (* TODO: this is actually a fmap on (A -> Prop) functor. *)
 Definition ltslang : S -> lang L := 
   fun s w => exists tr, w = labels tr /\ traces_at s tr.
+
+(* TODO: better name? *)
+Definition joint : rel (trace_seq S) := 
+  fun ts1 ts2 => 
+    match ts2 with 
+    | [::]    => true
+    | st :: _ => lst_state (src st) ts1 == src st
+    end.
 
 Definition mk_trace tr mkTr : trace :=
   mkTr (let: Trace _ trP := tr return is_trace tr in trP).
@@ -255,113 +266,190 @@ End EQ.
 
 Section Theory. 
 Context {L : Type} (S : ltsType L).
-Implicit Types (st : step S) (s : trace_seq S) (tr : trace S).
+Implicit Types (st : step S) (ts : trace_seq S) (tr : trace S).
 
-Lemma joint0s s :
-  joint [::] s.
-Proof. by rewrite /joint; case: s=> [|??] //=; rewrite rev_lnk. Qed.
+Lemma fst_state0 s :
+  fst_state s ([::] : trace_seq S) = s.
+Proof. by rewrite /fst_state /states (thead_head s) /=. Qed.
 
-Lemma joints0 s :
-  joint s [::].
-Proof. by rewrite /joint. Qed.    
+Lemma fst_state_cons s ts st :
+  fst_state s (st :: ts) = src st.
+Proof. by rewrite /fst_state (thead_head (src st)) /states /=. Qed.
 
-Lemma joint_cons st s1 s2 :
-  joint s1 (st :: s2) = joint s1 [:: st]. 
-Proof. by rewrite /joint; case: s2=> [|??] //=; rewrite last_rcons. Qed.
+Lemma fst_state_rcons s ts st :
+  fst_state s (rcons ts st) = if nilp ts then src st else fst_state s ts.
+Proof. by case: ts=> [|??] /=; rewrite fst_state_cons. Qed.
 
-Lemma joint_rcons st s1 s2 :
-  joint (rcons s1 st) s2 = joint [:: st] s2. 
-Proof. by rewrite /joint; case: s2=> [|??] //=; rewrite last_rcons. Qed.
+Lemma lst_state0 s :
+  lst_state s ([::] : trace_seq S) = s.
+Proof. by rewrite /lst_state /states (tlast_last s) /=. Qed.
 
-Lemma joint_lastE s st : 
-  joint s [:: st] = (last (src st) (states s) == src st).
+Lemma lst_state1 s st :
+  lst_state s ([:: st]) = dst st.
+Proof. by rewrite /lst_state /states (tlast_last s) /=. Qed.
+
+Lemma lst_state_rcons s ts st :
+  lst_state s (rcons ts st) = dst st.
 Proof. 
-  rewrite /joint /lnk /=.
-  case: (lastP s)=> [|{}s st'] //=.
-  rewrite last_rcons.
-  case: (nilp s)/nilP=> [->|Hnil] //=.
-  rewrite headI /states /=.
-  rewrite -behead_map map_rcons. 
-  move: Hnil; case: s => [|st'' {}s] //= _.
+  rewrite /lst_state (tlast_last (dst st)) /states /=.
+  rewrite headI /= last_map behead_rcons.
+  case: (nilp ts)/nilP=> [->|] //=.
   by rewrite last_rcons.
 Qed.
 
-Lemma cons_is_trace st s : 
-  is_step st -> joint [:: st] s -> is_trace s -> is_trace (st :: s).
+Lemma lst_state_cons s ts st :
+  lst_state s (st :: ts) = if nilp ts then dst st else lst_state s ts.
+Proof. 
+  move: st.
+  case: (lastP ts)=> [|{}ts st'] st /=.
+  - exact/lst_state1. 
+  rewrite lst_state_rcons; case: ifP=> [|_].
+  - by rewrite /nilp size_rcons. 
+  rewrite /lst_state (tlast_last (dst st')) /states /=.
+  by rewrite map_rcons last_rcons.
+Qed.
+
+Lemma lst_stateE st s ts :  
+  lst_state s ts = if nilp ts then s else dst (last st ts). 
+Proof. 
+  rewrite /lst_state /states.  
+  case: ts=> [|st' {}ts] //.
+  rewrite /nilp /=.
+  rewrite (tlast_last (dst st')) /=. 
+  by rewrite last_map.
+Qed.
+
+Lemma lst_stateNnil s s' ts : ts <> [::] ->
+  lst_state s' ts = lst_state s ts.
+Proof. 
+  case: ts=> [|st {}ts] //.
+  by rewrite !(lst_stateE st) /nilp /=.
+Qed.
+
+Lemma joint0s ts :
+  joint [::] ts.
+Proof. by rewrite /joint; case: ts=> [|??] //=. Qed.
+
+Lemma joints0 ts :
+  joint ts [::].
+Proof. by rewrite /joint. Qed.    
+
+Lemma joint_cons st ts1 ts2 :
+  joint ts1 (st :: ts2) = joint ts1 [:: st]. 
+Proof. by rewrite /joint; case: ts2=> [|??] //=; rewrite last_rcons. Qed.
+
+Lemma cons_joint st ts1 st' :
+  joint (st :: ts1) [:: st'] = lnk (last st ts1) st'. 
+Proof. 
+  rewrite /joint lst_state_cons.
+  rewrite (lst_stateE st).
+  by case: (nilp ts1)/nilP=> [->|].
+Qed.
+
+Lemma joint_rcons st ts1 ts2 :
+  joint (rcons ts1 st) ts2 = joint [:: st] ts2. 
+Proof. 
+  rewrite /joint; case: ts2=> [|st' {}ts2] //=. 
+  by rewrite -rcons0 !lst_state_rcons.
+Qed.
+
+Lemma joint_lastE ts st : 
+  joint ts [:: st] = (lst_state (src st) ts == src st).
+Proof. done. Qed.
+
+Lemma cons_is_trace st ts : 
+  is_step st -> joint [:: st] ts -> is_trace ts -> is_trace (st :: ts).
 Proof. 
   move=> Hs Hj Htr; rewrite /is_trace /=.
   repeat (apply/andP; split)=> //.
   - by move: Htr; rewrite /is_trace=> /andP[]. 
-  move: Hj Htr; case: s=> [|st' {}s] //=.
+  move: Hj Htr; case: ts=> [|st' {}ts] //=.
   rewrite joint_cons /joint /= => Hlnk.
   rewrite /is_trace /= => /andP[/andP[]].
   move=> ???; exact/andP.
 Qed.
 
-Lemma is_trace_rcons s st : 
-  is_trace (rcons s st) = [&& is_step st, is_trace s & joint s [:: st]].
+Lemma rcons_is_trace st ts : 
+  is_step st -> joint ts [:: st] -> is_trace ts -> is_trace (rcons ts st).
+Proof. 
+  move=> Hs Hj Htr; rewrite /is_trace /=.
+  repeat (apply/andP; split)=> //.
+  - rewrite all_rcons; apply/andP; split=> //.
+    by move: Htr; rewrite /is_trace=> /andP[].
+  move: Hj Htr; case: ts=> [|st' {}ts] //=.
+  rewrite /is_trace /= => + /andP[/andP[]].
+  rewrite cons_joint rcons_path=> ????; exact/andP.
+Qed.
+
+Lemma is_trace_rcons ts st : 
+  is_trace (rcons ts st) = [&& is_step st, is_trace ts & joint ts [:: st]].
 Proof. 
   rewrite /is_trace all_rcons -andbA -andbA.
-  apply/andb_id2l=> _; apply/andb_id2l=> _.
-  rewrite (sorted_rcons s (rev_lnk st)). 
-  by rewrite /joint.
+  rewrite (sorted_rcons ts (rev_lnk st)).
+  do 3 (apply/andb_id2l=> _).
+  rewrite /lnk joint_lastE. 
+  case: (lastP ts)=> [|{}ts st'].
+  - by rewrite lst_state0=> /=. 
+  by rewrite last_rcons lst_state_rcons.
 Qed.
+
+Lemma size_labels ts : 
+  size (labels ts) = size ts.
+Proof. by rewrite /labels size_map. Qed.
 
 Lemma labels_rcons s st : 
   labels (rcons s st) = rcons (labels s) (lbl st).
 Proof. by rewrite /labels map_rcons. Qed.
                          
-Lemma states_cons st s : joint [:: st] s ->
-  states (st :: s) = src st :: dst st :: behead (states s).
-Proof. admit. Admitted.
+(* Lemma states_cons st s : joint [:: st] s -> *)
+(*   states (st :: s) = src st :: dst st :: behead (states s). *)
+(* Proof. admit. Admitted. *)
     
-Lemma behead_states s :
-  behead (states s) = map dst s.
-Proof. by rewrite /states; case: s. Qed. 
+(* Lemma behead_states s : *)
+(*   behead (states s) = map dst s. *)
+(* Proof. by rewrite /states; case: s. Qed.  *)
 
-Lemma states_rcons_src s st : 
-  states (rcons s st) = (map src s) ++ [:: src st; dst st].
-Proof. admit. Admitted.
+(* Lemma states_rcons_src s st :  *)
+(*   states (rcons s st) = (map src s) ++ [:: src st; dst st]. *)
+(* Proof. admit. Admitted. *)
 
-Lemma states_rcons s st : ~~ nilp s -> is_trace s -> joint s [:: st] ->
-  states (rcons s st) = rcons (states s) (dst st).
+Lemma states_rcons s ts st : s = fst_state (src st) ts -> 
+  states s (rcons ts st) = rcons (states s ts) (dst st).
 Proof. 
-  move=> /(elimN nilP).
-  case: (lastP s)=> //=.
-  move=> {}s st' _.
-  rewrite is_trace_rcons=> /andP[Htr Hj]. 
-  rewrite joint_rcons /joint /= => Hlnk.
-  rewrite !states_rcons_src map_rcons.
-  rewrite -cats1 -cats1 -catA -catA /=.
-  by move: Hlnk; rewrite /lnk=> /eqP ->.
+  case: ts=> [|st' {}ts _] /=.
+  - by rewrite fst_state0=> ->. 
+  apply/eqP; rewrite !eqseq_cons. 
+  repeat (apply/andP; split=> //).
+  by rewrite map_rcons.
 Qed.
 
-Lemma head_states_rcons x s st : is_trace s -> joint s [:: st] ->
-  head x (states (rcons s st)) = if nilp s then src st else head x (states s).
-Proof. 
-  case: (nilp s)/nilP=> [->|Hnil] Htr Hj //=.
-  rewrite states_rcons //; last exact/nilP.
-  rewrite headI (headNnil x) //. 
-  admit.
-Admitted.
+(* Lemma head_states_rcons x s st : is_trace s -> joint s [:: st] -> *)
+(*   head x (states (rcons s st)) = if nilp s then src st else head x (states s). *)
+(* Proof.  *)
+(*   case: (nilp s)/nilP=> [->|Hnil] Htr Hj //=. *)
+(*   rewrite states_rcons //; last exact/nilP. *)
+(*   rewrite headI (headNnil x) //.  *)
+(*   admit. *)
+(* Admitted. *)
 
-Lemma last_states_rcons x s st : is_trace s -> joint s [:: st] ->
-  last x (states (rcons s st)) = dst st.
-Proof. 
-  case: (nilp s)/nilP=> [->|Hnil] Htr Hj //=.
-  rewrite states_rcons ?last_rcons //=; exact/nilP.
-Qed.
+(* Lemma last_states_rcons x s st : is_trace s -> joint s [:: st] -> *)
+(*   last x (states (rcons s st)) = dst st. *)
+(* Proof.  *)
+(*   case: (nilp s)/nilP=> [->|Hnil] Htr Hj //=. *)
+(*   rewrite states_rcons ?last_rcons //=; exact/nilP. *)
+(* Qed. *)
 
-Lemma states_cat s1 s2 : ~~ nilp s1 -> is_trace s1 -> joint s1 s2 -> 
-  states (s1 ++ s2) = states s1 ++ behead (states s2).
-Proof. 
-  rewrite behead_states; move=> /(elimN nilP).
-  move: s2; elim/last_ind: s1=> [|{}s1 st IH] s2 _ //=.
-  case: (nilp s1)/nilP=> [->|Hnil] //=.
-  rewrite is_trace_rcons=> /andP[Hs /andP[Htr Hj]].
-  rewrite joint_rcons cat_rcons IH //. 
-  rewrite states_rcons ?cat_rcons //=; exact/nilP.
-Qed.
+
+(* Lemma states_cat s1 s2 : ~~ nilp s1 -> is_trace s1 -> joint s1 s2 ->  *)
+(*   states (s1 ++ s2) = states s1 ++ behead (states s2). *)
+(* Proof.  *)
+(*   rewrite behead_states; move=> /(elimN nilP). *)
+(*   move: s2; elim/last_ind: s1=> [|{}s1 st IH] s2 _ //=. *)
+(*   case: (nilp s1)/nilP=> [->|Hnil] //=. *)
+(*   rewrite is_trace_rcons=> /andP[Hs /andP[Htr Hj]]. *)
+(*   rewrite joint_rcons cat_rcons IH //.  *)
+(*   rewrite states_rcons ?cat_rcons //=; exact/nilP. *)
+(* Qed. *)
 
 End Theory.
 
@@ -435,35 +523,41 @@ Proof.
   rewrite /ltslang /traces_at /=.
   rewrite /labels /= => /eqP Hh.
   suff: (exists (tr' : trace S), 
-           [/\ R (last s (states tr')) (last t (states tr)), 
+           [/\ R (lst_state s tr') (lst_state t tr), 
                labels tr = labels tr' 
-             & s == head s (states tr')
+             & s == fst_state s tr'
            ]).
   - by move=> [tr' []] ???; exists tr'.
   move: Htr Hh; elim/last_ind: tr=> [|{}tr st IH] /=.
   - by exists [trace] => /=.
-  rewrite is_trace_rcons=> /andP[Hs /andP[]].
-  move=> Htr Hj; rewrite head_states_rcons //.  
+  rewrite is_trace_rcons=> /andP[Hs /andP[Htr Hj]].
+  rewrite fst_state_rcons.
   case: (nilp tr)/nilP=> [->|Hnil] /=. 
   - admit.
   move=> Ht; move: (IH Htr Ht); clear IH. 
   move=> [tr' []] /[swap].
   rewrite !labels_rcons.    
   move: Hj; rewrite joint_lastE=> /eqP. 
-  rewrite (lastNnil t (src st)); last first.
-  - admit.
-  move: Hs=> + ->; rewrite /is_step=> Hs Hlbl HRl.
+  rewrite (lst_stateNnil t (src st))=> // ->. 
+  move: Hs; rewrite /is_step=> Hs Hlbl HRl.
   move: (sim_step HRl Hs)=> [s' []].
-  move=> HR' Hs' /eqP Hh.
-  pose st' := mk_step (lbl st) (last s (states tr')) s'.
+  move=> HR' Hs' /eqP Hfst.
+  have: ~~ nilp tr'.
+  - rewrite /nilp -size_labels -Hlbl size_labels. 
+    by move: Hnil=> /nilP.
+  move=> /nilP Hnil'.
+  pose st' := mk_step (lbl st) (lst_state s tr') s'.
   have Htr' : is_trace (rcons tr' st'). 
-  - admit.
+  - apply/rcons_is_trace=> //; last first. 
+    - exact/(valP tr').
+    rewrite joint_lastE /=.
+    by apply/eqP/lst_stateNnil.
   exists (Trace Htr')=> /=; split.
-  - admit.
-  - admit.
-  rewrite {1}Hh head_states_rcons //=.
-  2-3: admit.
-  case: (nilp tr')/nilP=> [->|] //.
+  - by rewrite !lst_state_rcons /=.
+  - by rewrite labels_rcons Hlbl.
+  rewrite fst_state_rcons. 
+  move: Hnil'=> /nilP /negbTE ->. 
+  exact/eqP/Hfst.  
 Admitted.
 
 End Theory.
